stdlib/lampe/Stdlib/Collections/BoundedVec.lean
@@ -1,32 +1,6 @@
-import «std-1.0.0-beta.12».Extracted.Collections.BoundedVec
-import «std-1.0.0-beta.12».Extracted.«std-1.0.0-beta.12»
+import «std-1.0.0-beta.12».Extracted
 import Lampe
 
 namespace Lampe.Stdlib.Collections.BoundedVec
 
-export «std-1.0.0-beta.12».Extracted (
-  «std::collections::bounded_vec::BoundedVec»
-  «std::collections::bounded_vec::BoundedVec::new»
-  «std::collections::bounded_vec::BoundedVec::get»
-  «std::collections::bounded_vec::BoundedVec::get_unchecked»
-  «std::collections::bounded_vec::BoundedVec::set»
-  «std::collections::bounded_vec::BoundedVec::set_unchecked»
-  «std::collections::bounded_vec::BoundedVec::push»
-  «std::collections::bounded_vec::BoundedVec::len»
-  «std::collections::bounded_vec::BoundedVec::max_len»
-  «std::collections::bounded_vec::BoundedVec::storage»
-  «std::collections::bounded_vec::BoundedVec::extend_from_array»
-  «std::collections::bounded_vec::BoundedVec::extend_from_slice»
-  «std::collections::bounded_vec::BoundedVec::extend_from_bounded_vec»
-  «std::collections::bounded_vec::BoundedVec::from_array»
-  «std::collections::bounded_vec::BoundedVec::pop»
-  «std::collections::bounded_vec::BoundedVec::any»
-  «std::collections::bounded_vec::BoundedVec::map»
-  «std::collections::bounded_vec::BoundedVec::mapi»
-  «std::collections::bounded_vec::BoundedVec::for_each»
-  «std::collections::bounded_vec::BoundedVec::for_eachi»
-  «std::collections::bounded_vec::BoundedVec::from_parts»
-  «std::collections::bounded_vec::BoundedVec::from_parts_unchecked»
-)
-
-open «std-1.0.0-beta.12».Extracted
+open «std-1.0.0-beta.12»
