stdlib/lampe/Stdlib/Hash/Poseidon2.lean
@@ -1,17 +1,6 @@
-import «std-1.0.0-beta.12».Extracted.Hash.Poseidon2
-import «std-1.0.0-beta.12».Extracted.«std-1.0.0-beta.12»
+import «std-1.0.0-beta.12».Extracted
 import Lampe
 
 namespace Lampe.Stdlib.Hash.Poseidon2
 
-export «std-1.0.0-beta.12».Extracted (
-  «std::hash::poseidon2::Poseidon2»
-  «std::hash::poseidon2::Poseidon2::hash»
-  «std::hash::poseidon2::Poseidon2::new»
-  «std::hash::poseidon2::Poseidon2::perform_duplex»
-  «std::hash::poseidon2::Poseidon2::absorb»
-  «std::hash::poseidon2::Poseidon2::squeeze»
-  «std::hash::poseidon2::Poseidon2::hash_internal»
-)
-
-open «std-1.0.0-beta.12».Extracted
+open «std-1.0.0-beta.12»
